# LaTeX {#sec-latex .unnumbered}

``` latex
R = 
\begin{pmatrix}
1 & r_0r & r_0r^2 & \cdots & r_0r^{T-1} \\
r_0r & 1 & r_0r & \cdots & r_0r^{T-2} \\
r_0r^2 & r_0r & 1 & \cdots & r_0r^{T-3} \\ 
\vdots & \vdots & \vdots & \vdots & \vdots \\ 
r_0r^{T-1} & r_0r^{T-2} & r_0r^{T-3} & \cdots & 1 
\end{pmatrix}
```

$$
R = 
\begin{pmatrix}
1 & r_0r & r_0r^2 & \cdots & r_0r^{T-1} \\
r_0r & 1 & r_0r & \cdots & r_0r^{T-2} \\
r_0r^2 & r_0r & 1 & \cdots & r_0r^{T-3} \\ 
\vdots & \vdots & \vdots & \vdots & \vdots \\ 
r_0r^{T-1} & r_0r^{T-2} & r_0r^{T-3} & \cdots & 1 
\end{pmatrix}
$$

\
\
\

``` latex
s(\\boldsymbol{\\hat{\\theta}}, y) = 
\begin{pmatrix} 
s(\hat{\theta}, y_1)_1 & s(\hat{\theta}, y_1)_2 & \cdots & s(\hat{\theta}, y_1)_k \\
\vdots & \vdots & \ddots & \vdots \\
s(\hat{\theta}, y_n)_1 & s(\hat{\theta}, y_n)_2 & \cdots & s(\hat{\theta}, y_n)_k \\
\end{pmatrix}
```

$$
s(\boldsymbol{\hat{\theta}}, y) = 
\begin{pmatrix} 
s(\hat{\theta}, y_1)_1 & s(\hat{\theta}, y_1)_2 & \cdots & s(\hat{\theta}, y_1)_k \\
\vdots & \vdots & \ddots & \vdots \\
s(\hat{\theta}, y_n)_1 & s(\hat{\theta}, y_n)_2 & \cdots & s(\hat{\theta}, y_n)_k \\
\end{pmatrix}
$$

\
\
\

``` latex
[1 \; x_{1t} \; x_{2t} \; \cdots \; x_{mt}] 
\cdot \left( \begin{array}{ccc} 
\hat{\beta}_{01} & \cdots & \hat{\beta}_{0k} \\ 
\vdots & \ddots & \vdots \\ 
\hat{\beta}_{m1} & \cdots & \hat{\beta}_{mk} \end{array} \right) 
= 
[\hat{y}_{t1} \; \hat{y}_{t2} \; \cdots \; \hat{y}_{tk}]
```

$$
[1 \; x_{1t} \; x_{2t} \; \cdots \; x_{mt}] 
\cdot \left( \begin{array}{ccc} 
\hat{\beta}_{01} & \cdots & \hat{\beta}_{0k} \\ 
\vdots & \ddots & \vdots \\ 
\hat{\beta}_{m1} & \cdots & \hat{\beta}_{mk} \end{array} \right) 
= 
[\hat{y}_{t1} \; \hat{y}_{t2} \; \cdots \; \hat{y}_{tk}]
$$

\
\
\

``` latex
ICC_{tt} = ICC_{tt'} = \frac {\sigma_b^2} {\sigma_b^2 + \sigma_e^2} r_{tt'}
```

$$
ICC_{tt} = ICC_{tt'} = \frac {\sigma_b^2} {\sigma_b^2 + \sigma_e^2} r_{tt'}
$$

\
\
\

``` latex
y_{ict} = \mu + \beta_0t + \beta_1X_{ct} + b_{ct} + e_{ict}
```

$$
y_{ict} = \mu + \beta_0t + \beta_1X_{ct} + b_{ct} + e_{ict}
$$

\
\
\

``` latex
\hat{\theta} = \arg\max_{\theta \in \Theta} \sum\_{i=1}^n w_i^{\text{forest}} \\cdot l(\theta; y_i)
```

$$
\hat{\theta} = \arg\max_{\theta \in \Theta} \sum_{i=1}^n w_i^{\text{forest}} \cdot l(\theta; y_i)
$$

\
\
\

``` latex
\begin{align*}
H(Y|X_1,\cdots, X_k) = \sum_{d = 0,1} \sum_{{i_1}=1}^c \cdots \sum_{{i_k}=1}^c \\
P(y_d | x_{i_1}, \cdots, x_{i_k}) \log P(y_d | x_{i_1}, \cdots, x_{i_k})
\end{align*}
```

$$
\begin{align*}
H(Y|X_1,\cdots, X_k) = \sum_{d = 0,1} \sum_{{i_1}=1}^c \cdots \sum_{{i_k}=1}^c \\
P(y_d | x_{i_1}, \cdots, x_{i_k}) \log P(y_d | x_{i_1}, \cdots, x_{i_k})
\end{align*}
$$

\
\
\

``` latex
\begin{align*}
x^2 + y^2 &= 1 \\
y &= \sqrt{1 - x^2}
\end{align*}
```

-   With the "&" symbols, the 2nd line stays lined up with the end of the first line

$$
\begin{align*}
x^2 + y^2 &= 1 \\
y &= \sqrt{1 - x^2}
\end{align*}
$$

\
\
\

``` latex
\begin{tabular} {lll}
Transformation & Function & Elasticity \\
\hline
Level Level & Y\;=\;a+bX & \epsilon = b \cdot \frac {X} {Y} \\  
Log Level & \log Y = a+bx & \epsilon = b \cdot X \\
Level-Log & Y = a + b \cdot \log X & \epsilon = \frac {b} {Y} \\
Log-Log & \log Y = a + b \cdot \log X & \epsilon = b \\
\hline
\end{tabular}
```

-   This is "Raw LaTeX" and will be ignored when the output is HTML. (See [Docs](https://quarto.org/docs/output-formats/pdf-basics.html#raw-latex))
-   In the last column, for some unknown reason, using `\frac` without another "\\" symbol before it throws an error. Adding `\epsilon =` to the expression made it work fine.

![](./_resources/LaTeX.resources/unknown_filename.7.png)

\
\
\

``` latex
c_{max}(t,\mu, \sigma) = \max \limits_{k = 1,..., dim(T)} \left | \frac {(t-\mu)_k} {\sqrt {\Sigma_{kk}}} \right |
```

-   Large absolute pipes require `\left`, `\right`
-   The text underneath "max" requires `\limits`

$$
c_{max}(t,\mu, \sigma) = \max \limits_{k = 1,..., dim(T)} \left | \frac {(t-\mu)_k} {\sqrt {\Sigma_{kk}}} \right |
$$

\
\
\

``` latex
\begin{align*}
\mbox{net present value (npv)} = &\sum \limits_{i = 0}^m benefit_i*(1-discount)^i -\\
&\sum \limits_{i=0}^m cost_i*(1-discount)^i
\end{align*}
```

$$
\begin{align*}
\mbox{net present value (npv)} = &\sum \limits_{i = 0}^m benefit_i*(1-discount)^i -\\
&\sum \limits_{i=0}^m cost_i*(1-discount)^i
\end{align*}
$$

\
\
\

``` latex
\epsilon_Z \stackrel{\text{iid}}{\sim} \mathcal{N}(0, 0.1)
```

$$
\epsilon_Z \stackrel{\text{iid}}{\sim} \mathcal{N}(0, 0.1)
$$

\
\
\

``` latex
\mbox{posterior} = \frac {\mbox{Prob of observed variables} \;\times\; \mbox{Prior}} {\mbox{Normalizing constant}}
```

$$
\mbox{posterior} = \frac {\mbox{Prob of observed variables} \;\times\; \mbox{Prior}} {\mbox{Normalizing constant}}
$$

\
\
\

``` latex
\lim\limits_{x \to +\infty} \sup \frac{\bar{F}(x)}{\bar{F}_{\exp}(x)} = \frac{\bar{F}(x)}{e^{-\lambda x}}, \;\; \forall \lambda > 0
```

$$
\lim\limits_{x \to +\infty} \sup \frac{\bar{F}(x)}{\bar{F}_{\exp}(x)} = \frac{\bar{F}(x)}{e^{-\lambda x}}, \;\; \forall \lambda > 0
$$

\
\
\

``` latex
\text{vec} = \left( \begin{array}{cc} \text{rand var1} \\
 \text {rand var2} \end{array} \right)
```

$$
\text{vec} = \left( \begin{array}{cc} \text{rand var1} \\
 \text {rand var2} \end{array} \right)
$$

\
\
\

``` latex
SBD(x,y) = 1 - \frac {\max (\text{NCCc}(x,y))} {\left\lVert x \right\rVert_2 \; \left\lVert y \right\rVert_2}
```

$$
SBD(x,y) = 1 - \frac {\max (\text{NCCc}(x,y))} {\left\lVert x \right\rVert_2 \; \left\lVert y \right\rVert_2}
$$

\
\
\

``` latex
D \not\!\perp\!\!\!\perp A \\
D \!\perp\!\!\!\perp A \\
Y \!\perp\!\!\!\perp X|Z
```

-   This one isn't rendering correctly in HTML

$$
D \not\!\perp\!\!\!\perp A\\
D \!\perp\!\!\!\perp A\\
Y \!\perp\!\!\!\perp X|Z
$$
